\begin{align}
F_0(\Ee) & = H_0(\Ee, J, J^\prime, 0) = F_1(\Ee, J, J^\prime, 0) 
	\!\!\! 
	& = &\; f_1(\Ee) 
	\nonumber \\
F_1(\Ee) & = H_1(\Ee, J, J^\prime, 0) = \textstyle F_4(\Ee, J, J^\prime, 0) \,+\! \frac{1}{3}F_7(\Ee, J, J^\prime, 0) 
	\!\!\! 
	& = &\; \textstyle f_4(\Ee) \,+\! \frac{1}{3}f_7(\Ee) 
	\nonumber \\
F_2(\Ee) & = H_2(\Ee, J, J^\prime, 0) = \textstyle F_{10}(\Ee, J, J^\prime, 0) \!+\! \frac{1}{2}F_{13}(\Ee, J, J^\prime, 0) 
	\!\!\! 
	& = &\; \textstyle f_{10}(\Ee) \!+\! \frac{1}{3}f_{13}(\Ee) 
	\nonumber \\
F_3(\Ee) & = H_3(\Ee, J, J^\prime, 0) = F_{18}(\Ee, J, J^\prime, 0) 
	\!\!\!
	& = &\; f_{18}(\Ee) .
\label{eq:holstein_FHFf}
\end{align}
